Refinery/Term/Extrinsic/Refinement/Beta.lean
@@ -15,16 +15,18 @@ variable {φ : Type u} {α : Type v} {ε : Type w} [S : Signature φ α ε]
 
 inductive DRWS.Beta : DRWS φ α
   | beta_pos {Γ Γl Γr : Ctx? α} {A : Ty α} {a b : Term φ (Ty α)}
-    (hΓ : Γ.SSplit Γl Γr) (da : Γr ⊢ a : A) (q : Quant) (hq : q ≤ quant Γr)
+    (hΓ : Γ.SSplit Γl Γr) (da : Γr ⊢ a : A) (q : Quant) (hq : q ⊓ quant A ≤ quant Γr)
     (db : Γl.cons ⟨A, q⟩ ⊢ b : B)
-    {el er} (ha : HasEff el a) (hb : HasEff er b) (he : el ⇀ er) (heq : q ≤ (pquant el).pos)
+    {el er} (ha : HasEff el a) (hb : HasEff er b) (he : el ⇀ er)
+    (heq : q ⊓ quant A ≤ (pquant el).pos)
     : Beta Γ B _ _
       (da.let₁ hΓ (db.pwk ((Ctx?.PWk.refl Γl).cons (by simp))))
       (db.subst (SubstDS.subst0 hΓ da q hq))
   | beta_neg {Γ Γl Γr : Ctx? α} {A : Ty α} {a b : Term φ (Ty α)}
-    (hΓ : Γ.SSplit Γl Γr) (da : Γr ⊢ a : A) (q : Quant) (hq : q ≤ quant Γr)
+    (hΓ : Γ.SSplit Γl Γr) (da : Γr ⊢ a : A) (q : Quant) (hq : q ⊓ quant A ≤ quant Γr)
     (db : Γl.cons ⟨A, q⟩ ⊢ b : B)
-    {el er} (ha : HasEff el a) (hb : HasEff er b) (he : el ↽ er) (heq : q ≤ (pquant el).neg)
+    {el er} (ha : HasEff el a) (hb : HasEff er b) (he : el ↽ er)
+    (heq : q ⊓ quant A ≤ (pquant el).neg)
     : Beta Γ B _ _
       (db.subst (SubstDS.subst0 hΓ da q hq))
       (da.let₁ hΓ (db.pwk ((Ctx?.PWk.refl Γl).cons (by simp))))
