Refinery/Term/Extrinsic/Wf/PreBeta.lean
@@ -13,9 +13,10 @@ variable  {φ : Type u} {α : Type v} {ε : Type w} [S : Signature φ α ε]
           {R : DRWS φ α}
 
 theorem Wf.pre_beta_pos  {Γ Γl Γr : Ctx? α} {A : Ty α}
-  (hΓ : Γ.SSplit Γl Γr) (a : Wf R Γr A) (q : Quant) (hq : q ≤ quant Γr)
+  (hΓ : Γ.SSplit Γl Γr) (a : Wf R Γr A) (q : Quant) (hq : q ⊓ quant A ≤ quant Γr)
   (b : Wf R (Γl.cons ⟨A, q⟩) B)
-  {el er} [ha : HasEff el a.tm] [hb : HasEff er b.tm] (he : el ⇀ er) (heq : q ≤ (pquant el).pos)
+  {el er} [ha : HasEff el a.tm] [hb : HasEff er b.tm] (he : el ⇀ er)
+  (heq : q ⊓ quant A ≤ (pquant el).pos)
   : a.let₁ hΓ (b.pwk ((Ctx?.PWk.refl Γl).cons (by simp))) ≤ b.subst (SubstDS.subst0 hΓ a.deriv q hq)
     := by
     apply DRWS.uniform.base
@@ -23,9 +24,10 @@ theorem Wf.pre_beta_pos  {Γ Γl Γr : Ctx? α} {A : Ty α}
     apply DRWS.Beta.beta_pos <;> assumption
 
 theorem Wf.pre_beta_neg {Γ Γl Γr : Ctx? α} {A : Ty α}
-    (hΓ : Γ.SSplit Γl Γr) (a : Wf R Γr A) (q : Quant) (hq : q ≤ quant Γr)
+    (hΓ : Γ.SSplit Γl Γr) (a : Wf R Γr A) (q : Quant) (hq : q ⊓ quant A ≤ quant Γr)
     (b : Wf R (Γl.cons ⟨A, q⟩) B)
-    {el er} [ha : HasEff el a.tm] [hb : HasEff er b.tm] (he : el ↽ er) (heq : q ≤ (pquant el).neg)
+    {el er} [ha : HasEff el a.tm] [hb : HasEff er b.tm] (he : el ↽ er)
+    (heq : q ⊓ quant A ≤ (pquant el).neg)
     : a.let₁ hΓ (b.pwk ((Ctx?.PWk.refl Γl).cons (by simp)))
     ≥ b.subst (SubstDS.subst0 hΓ a.deriv q hq)
     := by
@@ -34,15 +36,16 @@ theorem Wf.pre_beta_neg {Γ Γl Γr : Ctx? α} {A : Ty α}
     apply DRWS.Beta.beta_neg <;> assumption
 
 theorem Wf.pre_beta {Γ Γl Γr : Ctx? α} {A : Ty α}
-    (hΓ : Γ.SSplit Γl Γr) (a : Wf R Γr A) (q : Quant) (hq : q ≤ quant Γr)
+    (hΓ : Γ.SSplit Γl Γr) (a : Wf R Γr A) (q : Quant) (hq : q ⊓ quant A ≤ quant Γr)
     (b : Wf R (Γl.cons ⟨A, q⟩) B)
-    {el er} [ha : HasEff el a.tm] [hb : HasEff er b.tm] (he : el ⇌ er) (heq : q ≤ (pquant el))
+    {el er} [ha : HasEff el a.tm] [hb : HasEff er b.tm] (he : el ⇌ er)
+    (heq : q ⊓ quant A ≤ (pquant el))
     : a.let₁ hΓ (b.pwk ((Ctx?.PWk.refl Γl).cons (by simp)))
     ≈ b.subst (SubstDS.subst0 hΓ a.deriv q hq)
     := ⟨pre_beta_pos hΓ a q hq b he.left heq.left, pre_beta_neg hΓ a q hq b he.right heq.right⟩
 
 theorem Wf.pre_beta_pureIn {Γ Γl Γr : Ctx? α} {A : Ty α}
-    (hΓ : Γ.SSplit Γl Γr) (a : Wf R Γr A) (q : Quant) (hq : q ≤ quant Γr)
+    (hΓ : Γ.SSplit Γl Γr) (a : Wf R Γr A) (q : Quant) (hq : q ⊓ quant A ≤ quant Γr)
     (b : Wf R (Γl.cons ⟨A, q⟩) B)
     [ha : HasEff ⊥ a.tm]
     : a.let₁ hΓ (b.pwk ((Ctx?.PWk.refl Γl).cons (by simp)))
